SemanticsTernary/pfprefix_Predicates.thy
@@ -1,0 +1,77 @@
+theory pfprefix_Predicates
+imports
+  "../pfprefix_Firewall_Common"
+  "../pfprefix_Primitives"
+  pfprefix_Matching_Ternary
+begin
+fun all_match :: "('a \<Rightarrow> bool) \<Rightarrow> 'a match_expr  \<Rightarrow> bool" where
+"all_match _ MatchAny = True" |
+"all_match P (MatchNot m) = all_match P m" |
+"all_match P (MatchAnd m1 m2) = (all_match P m1 \<and> all_match P m2)" |
+"all_match P (Match m) = P m"
+
+definition no_ipv6 :: "common_primitive match_expr \<Rightarrow> bool" where
+"no_ipv6 mexpr =
+all_match (\<lambda>m. (case m of
+(Src (Hostspec (Address (IPv6 _)))) \<Rightarrow> False
+| (Dst (Address (IPv6 _))) \<Rightarrow> False
+| _ \<Rightarrow> True)) mexpr"
+
+definition no_af :: "common_primitive match_expr \<Rightarrow> bool" where
+"no_af mexpr = all_match (\<lambda>m. (case m of (Address_Family _) \<Rightarrow> False)) mexpr"
+
+definition good_match_expr :: "pfcontext \<Rightarrow> common_primitive match_expr \<Rightarrow> bool" where
+"good_match_expr ctx mexpr = all_match (good_primitive ctx) mexpr"
+
+fun all_AnchorRules_P :: "('a anchor_rule \<Rightarrow> bool) \<Rightarrow> 'a ruleset \<Rightarrow> bool" where
+"all_AnchorRules_P P rs = (\<forall> l \<in> set rs. (case l of (Anchor r b) \<Rightarrow> P r \<and> all_AnchorRules_P P b | _ \<Rightarrow> True))"
+
+fun all_AnchorRules_P' :: "('a anchor_rule \<Rightarrow> bool) \<Rightarrow> 'a ruleset \<Rightarrow> bool" where
+"all_AnchorRules_P' _ [] \<longleftrightarrow> True" |
+"all_AnchorRules_P' P ((PfRule r)#ls) \<longleftrightarrow> all_AnchorRules_P' P ls" |
+"all_AnchorRules_P' P ((Anchor r b)#ls) \<longleftrightarrow> P r \<and> all_AnchorRules_P' P b \<and> all_AnchorRules_P' P ls"
+
+lemma "all_AnchorRules_P P l= all_AnchorRules_P' P l"
+  by (induction P l rule: all_AnchorRules_P'.induct) auto
+
+lemma all_AnchorRules_append[simp]:
+  "all_AnchorRules_P P (xs @ ys) \<longleftrightarrow> all_AnchorRules_P P xs \<and> all_AnchorRules_P P ys"
+  by (induction P xs rule: all_AnchorRules_P.induct) auto
+
+definition no_anchors' :: "'a ruleset \<Rightarrow> bool" where
+"no_anchors' rs = all_AnchorRules_P (\<lambda>r. False) rs"
+
+lemma no_anchors_no_anchors'_eq:
+ "no_anchors rs \<longleftrightarrow> no_anchors' rs"
+  unfolding no_anchors'_def
+  by (induction rs) (auto split:line.splits)
+
+
+definition no_unknown_anchors :: "('a,'p) match_tac \<Rightarrow> 'a ruleset \<Rightarrow> bool" where
+"no_unknown_anchors \<gamma> rs = all_AnchorRules_P
+ (\<lambda>r. (\<forall> p. ternary_ternary_eval (map_match_tac (fst \<gamma>) p (anchor_rule.get_match r)) \<noteq> TernaryUnknown))
+ rs"
+
+
+fun all_PfRules_P :: "('a pf_rule \<Rightarrow> bool) \<Rightarrow> 'a ruleset \<Rightarrow> bool" where
+"all_PfRules_P P rs = (\<forall> l \<in> set rs. (case l of (PfRule r) \<Rightarrow> P r | (Anchor r b) \<Rightarrow> all_PfRules_P P b))"
+
+fun all_PfRules_P' :: "('a pf_rule \<Rightarrow> bool) \<Rightarrow> 'a ruleset \<Rightarrow> bool" where
+"all_PfRules_P' _ [] \<longleftrightarrow> True" |
+"all_PfRules_P' P ((PfRule r)#ls) \<longleftrightarrow> P r \<and> all_PfRules_P' P ls" |
+"all_PfRules_P' P ((Anchor r b)#ls) \<longleftrightarrow> all_PfRules_P' P b \<and> all_PfRules_P' P ls"
+
+lemma "all_PfRules_P P l= all_PfRules_P' P l"
+  by (induction P l rule: all_PfRules_P'.induct) auto
+
+lemma all_PfRules_append[simp]:
+  "all_PfRules_P P (xs @ ys) \<longleftrightarrow> all_PfRules_P P xs \<and> all_PfRules_P P ys"
+  by (induction P xs rule: all_PfRules_P.induct) auto
+
+definition no_match_quick :: "'a ruleset \<Rightarrow> bool" where
+"no_match_quick rs = all_PfRules_P (\<lambda>r. \<not>((pf_rule.get_action r) = ActionMatch \<and> pf_rule.get_quick r)) rs"
+
+
+definition good_ruleset :: "pfcontext \<Rightarrow> common_primitive ruleset \<Rightarrow> bool" where
+"good_ruleset ctx rs = (all_PfRules_P (\<lambda>r. good_match_expr ctx (pf_rule.get_match r)) rs \<and> all_AnchorRules_P (\<lambda>a. good_match_expr ctx (anchor_rule.get_match a)) rs)"
+end
